testing with refinement and graph theory

interface_abstraction/Scratch.thy
@@ -3,6 +3,7 @@ imports Main
 "../thy_lib/FiniteGraph"
 "../thy_lib/isabelle_afp/Graph_Theory/Pair_Digraph"
 "../thy_lib/Collections/Refine_Dflt"
+"../thy_lib/Collections/Examples/Autoref/Nested_DFS"
 begin
 
 
@@ -27,6 +28,13 @@ lemma fixes G::"'v graph" and Gafp::"('v, 'v \<times> 'v) pre_digraph"
   assumes transl: "Gafp = with_proj (graph_to_afp_graph G)"
   shows "has_directed_cycle G p = (\<exists>u. pre_digraph.awalk Gafp u p u \<and> distinct (tl (pre_digraph.awalk_verts Gafp u p)) \<and> p \<noteq> [])"
   by(simp add: has_directed_cycle_def pre_digraph.cycle_def transl)
+
+(*hmm, for my purposes, this almost looks executable enough! \<dots>*)
+definition pcycle :: "'v set \<Rightarrow> ('v \<times> 'v) set \<Rightarrow> 'v \<Rightarrow> bool" where
+  "pcycle V E v0 \<equiv> \<exists>v\<in>V. (v0,v)\<in>E\<^sup>* \<and> (v,v)\<in>E\<^sup>+"
+(*for my purpose, it might be enough:
+  (x,x) \<notin> view^+ but this does not find undirected cycles! *)
+(*is basic routing loop detection*)
 
 
 definition acyclic :: "('v, 'v \<times> 'v) pre_digraph \<Rightarrow> bool" where
@@ -72,6 +80,242 @@ lemma "acyclic \<lparr> pverts = {1::nat,2,3}, parcs = {(1,2),(2,3),(1,3)} \<rpa
 
 hide_const(open) succ (*my succ in my graph*)
 
+
+(*An undirected graph has a cycle if and only if a depth-first search (DFS) 
+  finds an edge that points to an already-visited vertex (a back edge) [wikipedia] *)
+(*need to trace edges!!*)
+
+(*http://www.geeksforgeeks.org/detect-cycle-undirected-graph/*)
+
+fun neighbors :: "('v \<times> 'v) list \<Rightarrow> 'v \<Rightarrow> 'v list" where
+  "neighbors E v = map (\<lambda> (_,y). y) (filter (\<lambda>(x,y). x=v) E)"
+
+declare neighbors.simps[simp del]
+
+lemma set_neighbors: "set (neighbors E v) = {y. (v,y) \<in> set E}"
+by (auto simp add: neighbors.simps)
+
+(* v0 \<Rightarrow> visited \<Rightarrow> parent \<Rightarrow> neighbors *)
+function x_cycle :: "'v \<Rightarrow> 'v list \<Rightarrow> 'v \<Rightarrow> (('v \<times> 'v) list) \<Rightarrow> bool" where
+  "x_cycle v visited parent E = ((neighbors E v \<noteq> []) \<and> (\<forall> nxt \<in> set (neighbors E v). (if nxt \<notin> set visited
+    then
+      x_cycle nxt (v#visited) v E
+    else
+      nxt \<noteq> parent)))"
+apply pat_completeness
+by auto
+
+(*how do I termination?*)
+termination x_cycle
+apply (relation "measure (\<lambda>(v,vis,p,E). Suc(length E) - length vis)")
+apply(simp)
+apply(simp only: set_neighbors)
+oops
+
+value "x_cycle (1::nat) [] 1 [(1,2), (2,3), (3,1)]"
+value "x_cycle (1::nat) [] 1 [(1,2), (2,3), (1,3)]"
+
+
+
+(*Tets with DFS AFP*)
+
+(*E should be a DAG, finds cycles in the underlying undirected graph
+*)
+(* E worklist visited*)
+function y_cycle :: "(('v \<times> 'v) list) \<Rightarrow> 'v list \<Rightarrow> 'v set \<Rightarrow> bool" where
+  "y_cycle E [] vis = False" |
+  "y_cycle E (w#ws) vis = (if w \<in> vis then True 
+                        else y_cycle E (neighbors E w@ws) (insert w vis))"
+by pat_completeness auto
+
+termination (*I HAVE NO IDEA how to do termination proofs ... Where is this documented?*)
+apply (relation "inv_image (finite_psubset <*lex*> less_than)  
+                   (\<lambda>(E,w,vis). ((fst ` set E \<union> snd ` set E) - vis, size w))")
+apply auto[1]
+apply (simp_all add: finite_psubset_def)
+apply(case_tac "w \<in> (fst ` set E \<union> snd ` set E)")
+apply(auto simp add: neighbors.simps)
+by (metis (lifting, mono_tags) filter_False imageI split_beta)
+
+
+value "y_cycle [(1,2), (2,3), (3,1)] [1::nat] {}"
+value "(1,1) \<in> {(1::nat,2::nat), (2,3), (3,1)}^+"
+value "y_cycle [(1,2), (2,3), (1,3)] [1::nat] {}"
+value "{(1::nat,2::nat), (2,3), (1,3)}^+"
+value "y_cycle [(1,2), (2,3), (3,4)] [1::nat] {}"
+value "y_cycle [(1,2), (2,1)] [1::nat] {}" (*not a DAG*)
+value "(1,1) \<in> {(1::nat,2::nat), (2,1)}^+"
+value "y_cycle [(1,1)] [1::nat] {}"
+value "y_cycle [(1,2), (1,3), (3,4), (1,5), (5,6), (2,4)] [1::nat] {}"
+
+
+
+(*
+How do I formalize that the underlying undirected graph is acyclic?
+Digraph.symmetric
+*)
+definition "underlying_undirected_cycle \<equiv> 
+\<exists>p u. awalk u p u \<and> distinct (tl (awalk_verts u p)) \<and> length p \<ge> 3"
+
+
+
+
+
+
+
+
+
+
+
+
+(*Collections&Refinement tests*)
+
+
+(*does this really detetc cycles?*)
+(*V=worklist, (vertex, parent)*)
+definition cycles_dfs_imp :: "('a \<Rightarrow>'a set) \<Rightarrow> 'a \<Rightarrow> bool nres" 
+  where
+  "cycles_dfs_imp succ v0 \<equiv>  do {
+      (_,_,cycle) \<leftarrow> WHILE (\<lambda> (V,Discovered,cycle). V \<noteq> {} \<and> \<not> cycle) (\<lambda> (V,Discovered,cycle). do {
+        (v,vparent) \<leftarrow> SPEC (\<lambda>v. v\<in>V );
+        let succs = (succ v) - {vparent};
+        if succs \<inter> fst ` Discovered  \<noteq> {} then RETURN (V,Discovered,True) else do {
+          let V = V - {(v,vparent)};
+          let Discovered = insert (v,vparent) Discovered;
+          let V = V \<union> ((succ v) \<times> {v});
+          RETURN (V,Discovered,cycle)
+        }
+      }) ({(v0,v0)},{},False);
+      RETURN cycle
+  }"
+
+(*everything reachable from V'*)
+lemma "{y. \<exists>x \<in> V'. (x,y) \<in> E\<^sup>*} = E\<^sup>*``V'" by blast
+
+definition cycles_dfs_imp_WHILE_invar :: "('v \<times> 'v) set \<Rightarrow> 'v \<Rightarrow> ('v\<times>'v) set \<times> ('v\<times>'v) set \<times> bool \<Rightarrow> bool" where
+  "cycles_dfs_imp_WHILE_invar E v0 \<sigma> \<equiv> let (V',Discovered,cycle) = \<sigma> in
+        V' \<subseteq> insert (v0,v0) E \<and> Discovered \<subseteq> insert (v0,v0) E \<and> 
+        E\<^sup>*``(fst ` V') \<union> fst ` Discovered = E\<^sup>*``{v0} \<and> 
+        ( Discovered \<inter> V' = {})"
+        (*{(a,b) \<in> E. a \<in> Discovered \<and> b \<in> Discovered} = E*)
+        (*need condition: no cycle so far!*)
+
+lemma cycles_dfs_imp_WHILE_invar_step1:
+  assumes "V = E\<^sup>*``{v0}" and "cycles_dfs_imp_WHILE_invar V E v0 (V',Discovered,cycle)"
+      "V' \<noteq> {}" "\<not> cycle" "x \<in> V'" "x \<in> Discovered"
+  shows "cycles_dfs_imp_WHILE_invar V E v0 (V', Discovered, True)"
+  using assms apply(simp add: cycles_dfs_imp_WHILE_invar_def) by blast
+
+lemma cycles_dfs_imp_WHILE_invar_step2:
+  assumes "V = E\<^sup>*``{v0}" and "cycles_dfs_imp_WHILE_invar V E v0 (V', Discovered, cycle)"
+       "V' \<noteq> {}" "\<not> cycle" "x \<in> V'" "x \<notin> Discovered"
+  shows "cycles_dfs_imp_WHILE_invar V E v0 (V' - {x} \<union> E `` {x}, insert x Discovered, cycle)"
+  using assms apply(simp add: cycles_dfs_imp_WHILE_invar_def)
+  apply(rule conjI)
+  apply blast
+  thm it_step_insert_iff
+oops
+
+lemma cycles_dfs_imp_WHILE_invar_goal_c1: 
+  assumes "V = E\<^sup>*``{v0}" and "cycles_dfs_imp_WHILE_invar V E v0 ({},Discovered,cycle)"
+  shows "\<not> cycle \<longleftrightarrow> (\<forall>x\<in>V. (v0, x) \<in> E\<^sup>* \<longrightarrow> (x, x) \<notin> E\<^sup>+)"
+  using assms by(auto simp add: cycles_dfs_imp_WHILE_invar_def)
+
+lemma cycles_dfs_imp_sound:
+  fixes succ and v0
+  defines "E \<equiv> {(v,v'). v'\<in>succ v}"
+  defines "V \<equiv> {v. (v0,v)\<in>E\<^sup>*}"
+  assumes F: "finite V"
+  shows "cycles_dfs_imp succ v0 \<le> SPEC (\<lambda>r. \<not> r \<longleftrightarrow> (\<forall>x\<in>V. (v0,x)\<in>E\<^sup>* \<longrightarrow> (x,x)\<notin>E\<^sup>+))"
+proof -
+  have S: "\<And>v. succ v = E``{v}"
+    by (auto simp: E_def)
+  have V: "V = E\<^sup>*``{v0}"
+    by (auto simp: V_def)
+  
+  from F show ?thesis
+    unfolding cycles_dfs_imp_def S
+    apply(intro WHILE_rule[where I="cycles_dfs_imp_WHILE_invar E v0"] refine_vcg)
+    apply(auto simp add: V_def cycles_dfs_imp_WHILE_invar_def)[1]
+    apply(clarify)
+    apply(drule(5) cycles_dfs_imp_WHILE_invar_step1[OF V])
+    apply(clarify)
+    prefer 2
+    apply(simp add: cycles_dfs_imp_WHILE_invar_goal_c1)
+    apply(auto simp add: V_def cycles_dfs_imp_WHILE_invar_def)[1]
+    oops
+
+
+
+(**The old version***)
+definition cycles_dfs_imp_WHILE_invar :: "'v set \<Rightarrow> ('v \<times> 'v) set \<Rightarrow> 'v \<Rightarrow> 'v set \<times> 'v set \<times> bool \<Rightarrow> bool" where
+  "cycles_dfs_imp_WHILE_invar V E v0 \<sigma> \<equiv> let (V',Discovered,cycle) = \<sigma> in
+        V' \<subseteq> V \<and> Discovered \<subseteq> V \<and> 
+        (*E\<^sup>*``V' = V - Discovered *) (*Discovered = V - E\<^sup>*``V'*) E\<^sup>*``V' \<union> Discovered = V \<and> 
+        ( Discovered \<inter> V' = {}) \<and>
+        ( \<not>cycle \<longleftrightarrow> (\<forall>x\<in>Discovered. (v0, x) \<in> E\<^sup>* \<longrightarrow> (x,x)\<notin>E\<^sup>+))"
+        (*{(a,b) \<in> E. a \<in> Discovered \<and> b \<in> Discovered} = E*)
+        (*need condition: no cycle so far!*)
+
+lemma cycles_dfs_imp_WHILE_invar_step1:
+  assumes "V = E\<^sup>*``{v0}" and "cycles_dfs_imp_WHILE_invar V E v0 (V',Discovered,cycle)"
+      "V' \<noteq> {}" "\<not> cycle" "x \<in> V'" "x \<in> Discovered"
+  shows "cycles_dfs_imp_WHILE_invar V E v0 (V', Discovered, True)"
+  using assms apply(simp add: cycles_dfs_imp_WHILE_invar_def) by blast
+
+lemma cycles_dfs_imp_WHILE_invar_step2:
+  assumes "V = E\<^sup>*``{v0}" and "cycles_dfs_imp_WHILE_invar V E v0 (V', Discovered, cycle)"
+       "V' \<noteq> {}" "\<not> cycle" "x \<in> V'" "x \<notin> Discovered"
+  shows "cycles_dfs_imp_WHILE_invar V E v0 (V' - {x} \<union> E `` {x}, insert x Discovered, cycle)"
+  using assms apply(simp add: cycles_dfs_imp_WHILE_invar_def)
+  apply(rule conjI)
+  apply blast
+  apply(rule conjI)oops
+apply (metis Image_singleton_iff rtrancl.rtrancl_into_rtrancl subsetD subsetI)
+  apply(rule conjI)
+  apply blast
+  apply(rule conjI)
+apply (metis Un_insert_left insert_Diff_single insert_subset rtrancl_apply_insert subsetI subset_antisym)
+  apply(rule conjI)defer 
+  apply(rule conjI)
+  oops
+  apply(rule conjI)
+  thm it_step_insert_iff
+oops
+
+lemma cycles_dfs_imp_WHILE_invar_goal_c1: 
+  assumes "V = E\<^sup>*``{v0}" and "cycles_dfs_imp_WHILE_invar V E v0 ({},Discovered,cycle)"
+  shows "\<not> cycle \<longleftrightarrow> (\<forall>x\<in>V. (v0, x) \<in> E\<^sup>* \<longrightarrow> (x, x) \<notin> E\<^sup>+)"
+  using assms by(auto simp add: cycles_dfs_imp_WHILE_invar_def)
+
+lemma cycles_dfs_imp_sound:
+  fixes succ and v0
+  defines "E \<equiv> {(v,v'). v'\<in>succ v}"
+  defines "V \<equiv> {v. (v0,v)\<in>E\<^sup>*}"
+  assumes F: "finite V"
+  shows "cycles_dfs_imp succ v0 \<le> SPEC (\<lambda>r. \<not> r \<longleftrightarrow> (\<forall>x\<in>V. (v0,x)\<in>E\<^sup>* \<longrightarrow> (x,x)\<notin>E\<^sup>+))"
+proof -
+  have S: "\<And>v. succ v = E``{v}"
+    by (auto simp: E_def)
+  have V: "V = E\<^sup>*``{v0}"
+    by (auto simp: V_def)
+  
+  from F show ?thesis
+    unfolding cycles_dfs_imp_def S
+    apply(intro WHILE_rule[where I="cycles_dfs_imp_WHILE_invar V E v0"] refine_vcg)
+    apply(auto simp add: V_def cycles_dfs_imp_WHILE_invar_def)[1]
+    apply(clarify)
+    apply(drule(5) cycles_dfs_imp_WHILE_invar_step1[OF V])
+    apply(clarify)
+    prefer 2
+    apply(simp add: cycles_dfs_imp_WHILE_invar_goal_c1)
+    apply(auto simp add: V_def cycles_dfs_imp_WHILE_invar_def)[1]
+    oops
+
+
+
+
+(*no idea what's wrong here*)
 definition cycles_dfs_rec :: "('a \<Rightarrow>'a set) \<Rightarrow> 'a \<Rightarrow> bool nres" 
   where
   "cycles_dfs_rec succ v0 \<equiv> REC (\<lambda>D (V,v). 
@@ -80,24 +324,30 @@ definition cycles_dfs_rec :: "('a \<Rightarrow>'a set) \<Rightarrow> 'a \<Righta
       let V=insert v V;
       FOREACH (succ v) (\<lambda>v' _. D (V,v')) False }
   ) ({},v0)"
-
-(*TODO only acyclic in reachable from v0*)
-
 lemma cycles_dfs_rec_sound:
-  fixes succ and G
+  fixes succ and v0
   defines "E \<equiv> {(v,v'). v'\<in>succ v}"
-  assumes F: "finite {v. (v0,v)\<in>E\<^sup>*}"
-  and wf_G: "wf_digraph G" and "arcs G = E"
-  shows "cycles_dfs_rec succ v0 \<le> SPEC (\<lambda>r. r \<longrightarrow> acyclic G)"
+  defines "V \<equiv> {v. (v0,v)\<in>E\<^sup>*}"
+  assumes F: "finite V"
+  shows "cycles_dfs_rec succ v0 \<le> SPEC (\<lambda>r. r \<longrightarrow> (\<forall>x\<in>V. (v0,x)\<in>E\<^sup>* \<longrightarrow> (x,x)\<notin>E\<^sup>+))"
 proof -
   have S: "\<And>v. succ v = E``{v}"
     by (auto simp: E_def)
   
   from F show ?thesis
-    unfolding cycles_dfs_rec_def S acyclic_alt[OF wf_G]
+    unfolding cycles_dfs_rec_def S
+    apply(intro REC_rule[where \<Phi>="\<lambda>(V',v'). (v0,v')\<in>E\<^sup>* \<and> V'\<subseteq>V \<and> (\<forall>x\<in>V'. (v0,x)\<in>E\<^sup>* \<longrightarrow> (x,x)\<notin>E\<^sup>+)"] 
+        FOREACH_rule[where I="\<lambda>Succs r. XXX"] refine_vcg) (*r \<longrightarrow> (\<forall>v\<in>V. (v0,v)\<in>E\<^sup>* \<longrightarrow> (v,v)\<notin>E\<^sup>+)*)
+    apply(refine_mono) (*REC is somehow undocumented*)
+    apply(simp)
+    apply(simp_all)
+    apply(rename_tac V' v')
+    apply(intro FOREACH_rule[where I="\<lambda>_ r. r \<longrightarrow> (\<forall>v\<in>V. (v0,v)\<in>E\<^sup>* \<longrightarrow> (v,v)\<notin>E\<^sup>+)"] refine_vcg)
+    apply(refine_rcg)
+    apply(auto)
     apply(refine_rcg refine_vcg impI REC_rule[where 
-        \<Phi>="\<lambda>(V,v). V \<subseteq> verts G \<and> (\<forall>x\<in>V. \<forall>y\<in>V. \<forall>p. pre_digraph.awalk G x p y \<longrightarrow> \<not> pre_digraph.cycle G p)"]
-        FOREACH_rule[where I="\<lambda>_ r. r \<longrightarrow> acyclic G"])
+        \<Phi>="\<lambda>(V,v). (v0,v)\<in>E\<^sup>* \<and> V\<subseteq>{v. (v0,v)\<in>E\<^sup>*} \<and> \<not>(\<exists>v\<in>V. (v0,v)\<in>E\<^sup>* \<and> (v,v)\<in>E\<^sup>+)"]
+        FOREACH_rule[where I="\<lambda>_ r. r \<longrightarrow> (\<forall>v\<in>V. (v0,v)\<in>E\<^sup>* \<longrightarrow> (v,v)\<notin>E\<^sup>+)"])
     apply(auto)
     apply(auto simp add: acyclic_alt[OF wf_G])
     (*apply (refine_rcg refine_vcg impI
@@ -108,6 +358,8 @@ proof -
     )*)
     apply(auto)
     oops
+
+(*TODO only acyclic in reachable from v0*)
 
 
 
